feat: congruent substitution

GroupoidModel/Russell_PER_MS/LemmasAutosubst.lean
@@ -7,8 +7,9 @@ This version uses `Autosubst.lean`. -/
 
 set_option grind.warning false
 
+-- TODO: generalize, or make a namespace and scope this
 /-- Proof by mutual induction on typing judgments. -/
-local macro "mutual_induction" : tactic =>
+macro "mutual_induction" : tactic =>
   `(tactic| (
     refine ⟨
       -- beautiful
@@ -53,7 +54,7 @@ local macro "mutual_induction" : tactic =>
 
 /-- Try solving each inductive case by its respective constructor passed to `grind`. -/
 -- TODO: can the script be shortened? metaprogram a generator for the cases?
-local macro "grind_cases" : tactic =>
+macro "grind_cases" : tactic =>
   `(tactic| (
     try case pi => grind [WfTp.pi]
     try case sigma => grind [WfTp.sigma]
@@ -119,20 +120,23 @@ theorem EqTm.le_univMax {Γ t u A l} : Γ ⊢[l] t ≡ u : A → l ≤ univMax :
 
 /-! ## Admissibility of renaming -/
 
-/-- The renaming `ξ : Δ ⟶ Γ` is well-formed. See `WfSb` for general substitutions. -/
+/-- The renaming `ξ : Δ ⟶ Γ` is well-formed. -/
 def WfRen (Δ : Ctx) (ξ : Nat → Nat) (Γ : Ctx) :=
   ∀ {i A l}, Lookup Γ i A l → Lookup Δ (ξ i) (A.rename ξ) l
 
 namespace WfRen
+
+theorem id (Γ) : WfRen Γ id Γ :=
+  fun lk => by convert lk; autosubst
 
 theorem wk (Γ A l) : WfRen ((A,l) :: Γ) Nat.succ Γ := by
   intro _ _ _ lk
   convert Lookup.succ _ _ lk
   autosubst
 
-theorem up {Δ Γ A ξ l} : WfRen Δ ξ Γ → Γ ⊢[l] A →
+theorem up {Δ Γ A ξ l} : WfRen Δ ξ Γ →
     WfRen ((A.rename ξ, l) :: Δ) (Expr.upr ξ) ((A, l) :: Γ) := by
-  intro wf _ _ _ _ lk
+  intro wf _ _ _ lk
   cases lk
   . rw [show (A.subst Expr.wk).rename (Expr.upr ξ) = (A.rename ξ).subst Expr.wk by autosubst]
     apply Lookup.zero
@@ -140,8 +144,9 @@ theorem up {Δ Γ A ξ l} : WfRen Δ ξ Γ → Γ ⊢[l] A →
     rw [show (A.subst Expr.wk).rename (Expr.upr ξ) = (A.rename ξ).subst Expr.wk by autosubst]
     apply Lookup.succ _ _ (wf lk)
 
-attribute [local grind] WfCtx.snoc in
-attribute [local grind] WfRen.up in
+end WfRen
+
+attribute [local grind] WfCtx.snoc WfRen.up in
 theorem rename_all :
     (∀ {Γ}, WfCtx Γ → True) ∧
     (∀ {Γ l A}, Γ ⊢[l] A →
@@ -163,74 +168,241 @@ theorem rename_all :
   -- Cases that didn't go through automatically.
   case snd => rw [ih_subst]; apply WfTm.snd <;> grind
   case cong_snd => rw [ih_subst]; apply EqTm.cong_snd <;> grind
-  case lam_app ihf _ _ Δwf ξwf => simpa only [autosubst] using EqTm.lam_app (ihf Δwf ξwf)
+  case lam_app =>
+    convert EqTm.lam_app .. using 1
+    . congr 2 <;> autosubst
+    all_goals grind
 
-end WfRen
+/-! ## Lookup well-formedness -/
+
+theorem WfCtx.lookup_wf {Γ i A l} : WfCtx Γ → Lookup Γ i A l → Γ ⊢[l] A := by
+  intro Γwf lk
+  induction lk
+  . rcases Γwf with _ | ⟨Γ, A⟩
+    rw [← Expr.ofRen_succ, ← Expr.rename_eq_subst_ofRen]
+    exact rename_all.2.1 A (Γ.snoc A) (WfRen.wk _ _ _)
+  . rename_i ih
+    rcases Γwf with _ | ⟨Γ, B⟩
+    rw [← Expr.ofRen_succ, ← Expr.rename_eq_subst_ofRen]
+    exact rename_all.2.1 (ih Γ) (Γ.snoc B) (WfRen.wk _ _ _)
 
 /-! ## Admissibility of substitution -/
 
-/-- The substitution `σ : Δ ⟶ Γ` is well-formed.
+/- Warning: notions defined in this namespace are suboptimal:
+they include tons of redundant assumptions
+needed to make the main induction go through.
 
-We use a functional definition as in the Autosubst paper.
+After substitution and inversion,
+we can define better versions with fewer arguments. -/
+namespace SubstProof
+
+/-- The substitution `σ : Δ ⟶ Γ` is well-formed
+and preserves bound variables' types.
+
+This is a functional definition as in the Autosubst paper,
+but with preservation data added for the inductive argument.
+
 A common alternative is to use an inductive characterization. -/
-def WfSb (Δ : Ctx) (σ : Nat → Expr) (Γ : Ctx) :=
-  ∀ {i A l}, Lookup Γ i A l → Δ ⊢[l] σ i : A.subst σ
+def IndWfSb (Δ : Ctx) (σ : Nat → Expr) (Γ : Ctx) :=
+  ∀ {i A l}, Lookup Γ i A l → (Δ ⊢[l] A.subst σ) ∧ (Δ ⊢[l] σ i : A.subst σ)
 
-namespace WfSb
+namespace IndWfSb
 
-theorem id {Γ} : WfCtx Γ → WfSb Γ Expr.bvar Γ := by
-  intro _ _ _ _ _
-  rw [Expr.subst_bvar, id_eq]
-  apply WfTm.bvar <;> assumption
+theorem ofRen {Δ Γ ξ} : WfCtx Δ → WfRen Δ ξ Γ → IndWfSb Δ (Expr.ofRen ξ) Γ := by
+  intro h h' _ _ _ lk
+  constructor
+  . rw [← Expr.rename_eq_subst_ofRen]
+    exact h.lookup_wf (h' lk)
+  . convert WfTm.bvar h (h' lk) using 1
+    autosubst
 
-theorem snoc {Δ Γ A t σ l} : WfSb Δ σ Γ → Γ ⊢[l] A → Δ ⊢[l] t : A.subst σ →
-    WfSb Δ (Expr.snoc σ t) ((A,l) :: Γ) := by
-  intro _ _ _ _ _ _ lk
-  cases lk <;> (autosubst; grind [WfSb])
+theorem id {Γ} : WfCtx Γ → IndWfSb Γ Expr.bvar Γ :=
+  fun h => ofRen h (WfRen.id Γ)
 
--- Note: the premise `Δ ⊢[l] A.subst σ` is needed to prove this before `subst_all`,
--- but is eliminated after. See `up`.
-theorem up' {Δ Γ A σ l} : WfCtx Δ → WfSb Δ σ Γ → Γ ⊢[l] A → Δ ⊢[l] A.subst σ →
-    WfSb ((A.subst σ, l) :: Δ) (Expr.up σ) ((A,l) :: Γ) := by
-  intro Δwf ΔσΓ _ ΔAσ _ _ _ lk
-  have ΔAσwf := WfCtx.snoc Δwf ΔAσ
+theorem wk {Γ A l} : WfCtx Γ → Γ ⊢[l] A → IndWfSb ((A,l) :: Γ) Expr.wk Γ :=
+  fun h h' => ofRen (h.snoc h') (WfRen.wk _ _ _)
+
+theorem snoc {Δ Γ A t σ l} : IndWfSb Δ σ Γ → Δ ⊢[l] A.subst σ → Δ ⊢[l] t : A.subst σ →
+    IndWfSb Δ (Expr.snoc σ t) ((A,l) :: Γ) := by
+  intro σ Aσ t _ _ _ lk
   cases lk
-  . apply WfTm.bvar ΔAσwf
-    convert Lookup.zero .. using 1
-    autosubst
-  . rename_i lk
-    convert WfRen.rename_all.2.2.2.1 (ΔσΓ lk) ΔAσwf (@WfRen.wk Δ (A.subst σ) l) using 1
-    autosubst
+  . constructor
+    . convert Aσ using 1; autosubst
+    . autosubst; grind [IndWfSb]
+  next lk =>
+    constructor
+    . convert (σ lk).1 using 1; autosubst
+    . autosubst; grind [IndWfSb]
 
-attribute [local grind] WfCtx.snoc in
-attribute [local grind] WfSb.up' in
+theorem up_of_eq {Δ Γ A Aσ σ l} : WfCtx Δ → IndWfSb Δ σ Γ →
+    Δ ⊢[l] Aσ → Δ ⊢[l] A.subst σ → Δ ⊢[l] Aσ ≡ A.subst σ →
+    IndWfSb ((Aσ, l) :: Δ) (Expr.up σ) ((A,l) :: Γ) := by
+  intro Δwf ΔσΓ ΔAσ ΔAσ' ΔAσeq _ _ _ lk
+  have ΔAσwf := Δwf.snoc ΔAσ
+  cases lk
+  . constructor
+    . convert rename_all.2.1 ΔAσ' ΔAσwf (@WfRen.wk _ _ _) using 1 <;> autosubst
+    . apply WfTm.conv (A := Aσ.subst Expr.wk)
+      . apply WfTm.bvar ΔAσwf
+        apply Lookup.zero
+      . convert rename_all.2.2.1 ΔAσeq ΔAσwf (@WfRen.wk _ _ _) using 1 <;> autosubst
+  next lk =>
+    constructor
+    . convert rename_all.2.1 (ΔσΓ lk).1 ΔAσwf (@WfRen.wk _ _ _) using 1 <;> autosubst
+    . convert rename_all.2.2.2.1 (ΔσΓ lk).2 ΔAσwf (@WfRen.wk _ _ _) using 1
+      autosubst
+
+theorem up {Δ Γ A σ l} : WfCtx Δ → IndWfSb Δ σ Γ → Δ ⊢[l] A.subst σ →
+    IndWfSb ((A.subst σ, l) :: Δ) (Expr.up σ) ((A,l) :: Γ) :=
+  fun Δwf ΔσΓ ΔAσ => up_of_eq Δwf ΔσΓ ΔAσ ΔAσ (EqTp.refl_tp ΔAσ)
+
+end IndWfSb
+
+/-- The substitutions `σ σ' : Δ ⟶ Γ` are definitionally equal,
+preserve variables' types, and are congruent on those types.
+See also `IndWfSb`. -/
+def IndEqSb (Δ : Ctx) (σ σ' : Nat → Expr) (Γ : Ctx) :=
+  ∀ {i A l}, Lookup Γ i A l →
+    (Δ ⊢[l] A.subst σ) ∧ (Δ ⊢[l] A.subst σ') ∧ (Δ ⊢[l] A.subst σ ≡ A.subst σ') ∧
+    (Δ ⊢[l] σ i ≡ σ' i : A.subst σ)
+
+namespace IndEqSb
+
+theorem refl {Δ Γ σ} : IndWfSb Δ σ Γ → IndEqSb Δ σ σ Γ :=
+  fun h _ _ _ lk => ⟨(h lk).1, (h lk).1, EqTp.refl_tp (h lk).1, EqTm.refl_tm (h lk).2⟩
+
+theorem symm {Δ Γ σ σ'} : IndEqSb Δ σ σ' Γ → IndEqSb Δ σ' σ Γ := by
+  grind [IndEqSb, EqTp.symm_tp, EqTm.symm_tm, EqTm.conv_tm]
+
+theorem trans {Δ Γ σ σ' σ''} : IndEqSb Δ σ σ' Γ → IndEqSb Δ σ' σ'' Γ → IndEqSb Δ σ σ'' Γ :=
+  fun h h' _ _ _ lk => ⟨
+    (h lk).1,
+    (h' lk).2.1,
+    (h lk).2.2.1.trans_tp (h' lk).2.2.1,
+    (h lk).2.2.2.trans_tm (h lk).1 ((h' lk).2.2.2.conv_tm (h lk).2.2.1.symm_tp)
+  ⟩
+
+theorem snoc {Δ Γ A t t' σ σ' l} : IndEqSb Δ σ σ' Γ →
+    Δ ⊢[l] A.subst σ → Δ ⊢[l] A.subst σ' → Δ ⊢[l] A.subst σ ≡ A.subst σ' →
+    Δ ⊢[l] t ≡ t' : A.subst σ →
+    IndEqSb Δ (Expr.snoc σ t) (Expr.snoc σ' t') ((A,l) :: Γ) := by
+  intro σσ' Aσ Aσ' AσAσ' tt' _ _ _ lk
+  cases lk
+  . repeat any_goals apply And.intro
+    . convert Aσ using 1; autosubst
+    . convert Aσ' using 1; autosubst
+    . convert AσAσ' using 1 <;> autosubst
+    . convert tt' using 1; autosubst
+  next lk =>
+    repeat any_goals apply And.intro
+    . convert (σσ' lk).1 using 1; autosubst
+    . convert (σσ' lk).2.1 using 1; autosubst
+    . convert (σσ' lk).2.2.1 using 1 <;> autosubst
+    . convert (σσ' lk).2.2.2 using 1 <;> autosubst
+
+theorem up {Δ Γ A σ σ' l} : WfCtx Δ → IndEqSb Δ σ σ' Γ →
+    Δ ⊢[l] A.subst σ → Δ ⊢[l] A.subst σ' → Δ ⊢[l] A.subst σ ≡ A.subst σ' →
+    IndEqSb ((A.subst σ, l) :: Δ) (Expr.up σ) (Expr.up σ') ((A,l) :: Γ) := by
+  intro Δwf ΔσΓ ΔAσ ΔAσ' ΔAσeq _ _ _ lk
+  have ΔAσwf := Δwf.snoc ΔAσ
+  cases lk
+  . repeat any_goals apply And.intro
+    . convert rename_all.2.1 ΔAσ ΔAσwf (@WfRen.wk _ _ _) using 1 <;> autosubst
+    . convert rename_all.2.1 ΔAσ' ΔAσwf (@WfRen.wk _ _ _) using 1 <;> autosubst
+    . convert rename_all.2.2.1 ΔAσeq ΔAσwf (@WfRen.wk _ _ _) using 1 <;> autosubst
+    . apply EqTm.refl_tm
+      apply WfTm.bvar ΔAσwf
+      convert Lookup.zero .. using 1
+      autosubst
+  next lk =>
+    have := ΔσΓ lk
+    repeat any_goals apply And.intro
+    . convert rename_all.2.1 this.1 ΔAσwf (@WfRen.wk _ _ _) using 1 <;> autosubst
+    . convert rename_all.2.1 this.2.1 ΔAσwf (@WfRen.wk _ _ _) using 1 <;> autosubst
+    . convert rename_all.2.2.1 this.2.2.1 ΔAσwf (@WfRen.wk _ _ _) using 1 <;> autosubst
+    . convert rename_all.2.2.2.2 this.2.2.2 ΔAσwf (@WfRen.wk Δ (A.subst σ) l) using 1 <;>
+        autosubst
+
+end IndEqSb
+
+attribute [local grind] WfCtx.snoc IndWfSb.up_of_eq IndWfSb.up IndEqSb.up in
 theorem subst_all :
     (∀ {Γ}, WfCtx Γ → True) ∧
     (∀ {Γ l A}, Γ ⊢[l] A →
-      ∀ {Δ σ}, WfCtx Δ → WfSb Δ σ Γ → Δ ⊢[l] A.subst σ) ∧
+      ∀ {Δ σ}, WfCtx Δ → IndWfSb Δ σ Γ →
+        (Δ ⊢[l] A.subst σ) ∧
+          ∀ {σ'}, IndWfSb Δ σ' Γ → IndEqSb Δ σ σ' Γ →
+            Δ ⊢[l] A.subst σ ≡ A.subst σ') ∧
     (∀ {Γ l A B}, Γ ⊢[l] A ≡ B →
-      ∀ {Δ σ}, WfCtx Δ → WfSb Δ σ Γ → Δ ⊢[l] A.subst σ ≡ B.subst σ) ∧
+      ∀ {Δ σ σ'}, WfCtx Δ → IndWfSb Δ σ Γ → IndWfSb Δ σ' Γ → IndEqSb Δ σ σ' Γ →
+        Δ ⊢[l] A.subst σ ≡ B.subst σ') ∧
     (∀ {Γ l t A}, Γ ⊢[l] t : A →
-      ∀ {Δ σ}, WfCtx Δ → WfSb Δ σ Γ → Δ ⊢[l] t.subst σ : A.subst σ) ∧
+      ∀ {Δ σ}, WfCtx Δ → IndWfSb Δ σ Γ →
+        (Δ ⊢[l] t.subst σ : A.subst σ) ∧
+          ∀ {σ'}, IndWfSb Δ σ' Γ → IndEqSb Δ σ σ' Γ →
+            Δ ⊢[l] t.subst σ ≡ t.subst σ' : A.subst σ) ∧
     (∀ {Γ l t u A}, Γ ⊢[l] t ≡ u : A →
-      ∀ {Δ σ}, WfCtx Δ → WfSb Δ σ Γ → Δ ⊢[l] t.subst σ ≡ u.subst σ : A.subst σ) := by
-  -- This goes through using the same proof as renaming!
+      ∀ {Δ σ σ'}, WfCtx Δ → IndWfSb Δ σ Γ → IndWfSb Δ σ' Γ → IndEqSb Δ σ σ' Γ →
+        Δ ⊢[l] t.subst σ ≡ u.subst σ' : A.subst σ) := by
   have ih_subst (B a : Expr) (σ) :
       (B.subst a.toSb).subst σ = (B.subst (Expr.up σ)).subst (a.subst σ).toSb := by autosubst
   mutual_induction
   case snoc => exact True.intro
   all_goals try dsimp [Expr.subst] at *
-  case bvar => grind [WfSb]
+  case bvar => grind [IndWfSb, IndEqSb]
   grind_cases
-  case snd => rw [ih_subst]; apply WfTm.snd <;> grind
+  case pi => grind [WfTp.pi, EqTp.cong_pi]
+  case sigma => grind [WfTp.sigma, EqTp.cong_sigma]
+  case univ => grind [WfTp.univ, EqTp.refl_tp]
+  case el => grind [WfTp.el, EqTp.cong_el]
+  case symm_tp => grind [IndEqSb.symm, EqTp.symm_tp]
+  case trans_tp => grind [EqTp.trans_tp, IndEqSb.trans, IndEqSb.refl]
+  case lam => grind [WfTm.lam, EqTm.cong_lam]
+  case app => grind [WfTm.app, EqTm.cong_app]
+  case pair => grind [WfTm.pair, EqTm.cong_pair]
+  case fst => grind [WfTm.fst, EqTm.cong_fst]
+  case snd =>
+    constructor
+    . rw [ih_subst]; apply WfTm.snd <;> grind
+    . intros; rw [ih_subst]; apply EqTm.cong_snd <;> grind
+  case code => grind [WfTm.code, EqTm.cong_code]
+  case conv => grind [WfTm.conv, EqTm.conv_tm, IndEqSb.refl]
+  case app_lam =>
+    rw [ih_subst, ih_subst]
+    apply (EqTm.app_lam ..).trans_tm
+    . autosubst; grind [IndWfSb.snoc]
+    . autosubst
+      rename_i iht _ _ _ _ _ _ _ _
+      apply (iht ..).2
+      . grind [IndWfSb.snoc]
+      . grind [IndEqSb.snoc]
+      . grind
+      . grind [IndWfSb.snoc]
+    all_goals grind
+  case fst_pair => apply (EqTm.fst_pair ..).trans_tm <;> grind
+  case snd_pair =>
+    rw [ih_subst]; apply (EqTm.snd_pair ..).trans_tm
+    . autosubst; grind [IndWfSb.snoc]
+    all_goals grind
+  case lam_app ihA ihB ihf _ _ _ Δ σ σ' σσ' =>
+    apply (ihf Δ σ |>.2 σ' σσ').trans_tm (by grind [WfTp.pi])
+    have := EqTm.lam_app
+      (ihA Δ σ').1
+      (ihB (Δ.snoc (by grind))
+      (σ'.up Δ (by grind))).1
+      (ihf Δ σ').1
+    convert this.conv_tm _ using 3 <;> autosubst
+    grind [EqTp.cong_pi, IndEqSb.symm, Expr.up_eq_snoc]
+  case pair_fst_snd =>
+    apply (EqTm.pair_fst_snd ..).trans_tm <;>
+      grind [WfTp.sigma, EqTm.cong_pair, EqTm.cong_fst, EqTm.cong_snd]
+  case conv_tm => grind [EqTm.conv_tm, IndEqSb.refl]
+  case symm_tm => grind [EqTm.symm_tm, EqTm.conv_tm, IndEqSb.symm]
+  case trans_tm => grind [EqTm.trans_tm, EqTm.conv_tm, IndEqSb.trans, IndEqSb.refl]
   case cong_snd => rw [ih_subst]; apply EqTm.cong_snd <;> grind
-  case lam_app ihf _ _ Δwf ξwf => simpa only [autosubst] using EqTm.lam_app (ihf Δwf ξwf)
 
-theorem up {Δ Γ A σ l} : WfCtx Δ → WfSb Δ σ Γ → Γ ⊢[l] A →
-    WfSb ((A.subst σ, l) :: Δ) (Expr.up σ) ((A,l) :: Γ) :=
-  fun h₁ h₂ h₃ => up' h₁ h₂ h₃ (subst_all.2.1 h₃ h₁ h₂)
+end SubstProof
 
-end WfSb
 
 theorem WfTp.subst {Δ Γ A σ l} : Γ ⊢[l] A → WfCtx Δ → WfSb Δ σ Γ → Δ ⊢[l] A.subst σ :=
   fun h h₁ h₂ => WfSb.subst_all.2.1 h h₁ h₂
